compiler/pollang/ReflexKState.v
@@ -60,3 +60,186 @@ Definition HANDLERS : handlers (VVD := PAY_DESC) KST_DESC :=
       match bad with end
     end (pay m)
   ).
+
+Require Import PolLang.
+Require Import ActionMatch.
+Require Import Tactics.
+Require Import ReflexFin.
+Require Import List.
+
+Ltac destruct_msg :=
+  match goal with
+  (*Tag is Some False*)
+  | [ f : False |- _ ]
+      => destruct f
+  | [ pay : s[[lkup_tag (Some ?f)]] |- _ ]
+      => match type of f with
+         | option _ => destruct f; destruct_msg
+         end
+  | [ pay : s[[lkup_tag _]] |- _ ]
+      => destruct pay; simpl in *; destruct_msg
+  | [ a : prod _ _ |- _ ]
+      => destruct a; simpl in *; destruct_msg
+  | [ tag : fin _ |- _ ]
+      => destruct tag; destruct_msg
+  | [ m : msg |- _ ]
+      => destruct m; destruct_msg
+  | _
+    => idtac
+  end.
+
+(*Destructs num, str, or fd equalities in the context.*)
+Ltac destruct_eq hdlrs H :=
+  unfold hdlrs in H; simpl in H;
+  match type of H with
+  | context[num_eq ?a ?b]
+    => destruct (num_eq a b); simpl in *; destruct_eq hdlrs H
+  | context[str_eq ?a ?b]
+    => destruct (str_eq a b); simpl in *; destruct_eq hdlrs H
+  | context[fd_eq ?a ?b]
+    => destruct (fd_eq a b); simpl in *; destruct_eq hdlrs H
+  | _
+    => idtac
+  end.
+
+Require Import Ynot.
+    Ltac unpack :=
+  match goal with
+  | [ s : kstate _, H : ?s = _, s' : kstate _,
+      H' : ?s' = kstate_run_prog ?KST_DESC _ _ _ ?s _ |- _ ]
+      => rewrite H in H'; (*apply f_equal with (f:=ktr KST_DESC) in H';
+         unfold handlers in H'; simpl in H';*) rewrite H' in *; simpl in *; unpack
+  | [ s : init_state _ _, H : ?s = _ |- _ ]
+      (*This is problematic because it destroys information about s*)
+      => rewrite H in *; simpl in *; unpack
+  | [ H: [_]%inhabited = [_]%inhabited |- _ ]
+      => apply pack_injective in H;
+         rewrite -> H || rewrite <- H
+  end.
+
+(*Erases hypothesis relating to old states on which we are not performing induction.*)
+(*First rewrites those states to avoid losing information.*)
+Ltac clear_old_hyps :=
+  match goal with
+  | [ s : kstate _, s' : kstate _, tr : KTrace |- _ ]
+      => match goal with
+         | [ H : s = _, H' : s' = _, H'' : tr = _,
+             IHReach : forall tr : KTrace, _ |- _ ]
+           => try rewrite H in *; try rewrite H' in *;
+              clear dependent s; clear dependent s';
+              clear dependent tr; clear IHReach
+         end
+  end.
+
+Ltac destruct_unpack :=
+  match goal with
+  | [ m : msg, H : _ = kstate_run_prog _ _ _ _ _ _,
+      H' : Reach _ _ _ ?HDLRS _ |- _ ]
+      => destruct_msg; destruct_eq HDLRS H; unpack
+  | [ m : msg |- _ ]
+      => destruct_msg; unpack
+  | _
+      => unpack
+  end.
+
+Ltac subst_states :=
+  match goal with 
+  | [ s : kstate _ |- _ ]
+      => match goal with
+         | [ _ : s = _ |- _ ]
+             => subst s; subst_states
+         end
+  | _
+      => idtac
+  end.
+
+Ltac subst_assignments :=
+  match goal with
+  | [ a := _ |- _ ]
+      => subst a; subst_assignments
+  | _
+      => idtac
+  end.
+
+Ltac use_IH :=
+  match goal with
+  | [ IHReach : ?H -> ?rest, H' : ?H, _ : ktr _ ?s = inhabits ?tr |- _ ]
+    => match rest with
+       | context[forall tr' : KTrace, ktr _ s = inhabits tr' -> _]
+          => let act := fresh "act" in
+             let H'' := fresh "H" in
+             apply IHReach with (tr':=tr) in H'; auto;
+             (*TODO: What if there is more than one hypothesis?*)
+             destruct H' as [ act H'' ]; exists act; tauto
+       end
+  end.
+
+Ltac releaser_match :=
+    match goal with
+    | [ |- context[ In _ (?act::_) ] ]
+      => exists act; compute; tauto
+    | [ |- context[ In _ (_::?act::_) ] ]
+      => exists act; compute; tauto
+    | [ |- context[ In _ (_::_::?act::_) ] ]
+      => exists act; compute; tauto
+    | [ |- exists past, (?act = past \/ _ ) /\ _ ]
+      => exists act; compute; tauto
+    | [ |- exists past, (_ \/ ?act = past \/ _ ) /\ _ ]
+      => exists act; compute; tauto
+    | [ |- exists past, (_ \/ _ \/ ?act = past \/ _ ) /\ _ ]
+      => exists act; compute; tauto
+    | [ |- exists past, (_ \/ _ \/ _ \/ ?act = past \/ _ ) /\ _ ]
+      => exists act; compute; tauto
+    end.
+
+Ltac exists_past :=
+  clear_old_hyps;
+  match goal with
+  | [ _ : ktr _ _ = inhabits ?tr, H : Reach _ _ _ _ _ |- _ ]
+      => generalize dependent tr; induction H; simpl in *; intros
+  end;
+  match goal with
+  | [ H : _ = initial_init_state _ _ |- _ ]
+      => rewrite H in *; intuition (*Initial state. Contradiction?*)
+  | _
+      => destruct_unpack; subst_assignments; subst_states;
+         simpl in *; try contradiction; try releaser_match; try use_IH
+         (*destruct_eq might have created contradictions
+           with previous calls of destruct_eq*)
+  end.
+
+Ltac match_releases :=
+  match goal with
+  | [ |- Release _ _ _ _ nil ]
+      => constructor
+  | [ H : ktr _ ?s = inhabits ?tr,
+      IH : forall tr', inhabits tr' = ktr _ ?s ->
+                       Release _ _ ?past ?future tr'
+                       |- Release _ _ ?past ?future ?tr ]
+      => auto
+  | [ H : AMatch ?future ?act |- Release ?nb_msg ?pdv _ ?future (?act::_) ]
+      => apply R_future; [ match_releases | exists_past ]
+  | [ H : ~AMatch ?future ?act |- Release ?nb_msg ?pdv _ ?future (?act::_) ]
+      => apply R_not_future; [ match_releases | assumption ]
+  | [ |- Release ?nb_msg ?pdv _ ?future (?act::_) ]
+      => let H := fresh "H" in
+         pose proof (decide_act nb_msg pdv future act) as H;
+         destruct H; try contradiction; match_releases
+  end.
+
+Theorem release : forall st tr u,
+  Reach _ _ INIT HANDLERS st -> inhabits tr = ktr _ st ->
+  Release NB_MSG PAY_DESC
+          (@KORecv NB_MSG PAY_DESC None
+                   (Some (@Build_opt_msg NB_MSG PAY_DESC
+                                         (Some None) (None, (None, tt)))))
+          (@KOSend NB_MSG PAY_DESC None
+                   (Some (@Build_opt_msg NB_MSG PAY_DESC
+                                         None (Some u, tt))))
+          tr.
+Proof.
+  intros.
+  generalize dependent tr.
+  induction H; simpl in *; intros;
+  destruct_unpack; match_releases.
+Qed.
